raw lambda

Affine/Basic.lean
@@ -1,5 +1,6 @@
 import Mathlib.Data.Nat.Basic
 import Mathlib.Data.Finset.Basic
+import Mathlib.Data.Multiset.Sort
 
 /--
   Affine lambda terms, where bound variables can be used at most once.
@@ -8,24 +9,34 @@ import Mathlib.Data.Finset.Basic
   - `List`: Can have duplicates.
   - `Set`: Can be infinite.
 -/
-inductive Affine : (vs : Finset String) → Type
-| var (x : String) : Affine {x}
-| abs (x : String) (e : Affine vs) : Affine (vs \ {x})
+inductive Affine : (vs : Finset ℕ) → Type
+| var (x : ℕ) : Affine {x}
+| abs (x : ℕ) (e : Affine vs) : Affine (vs \ {x})
 | app (e₁ : Affine vs₁) (e₂ : Affine vs₂) (h : vs₁ ∩ vs₂ = ∅) : Affine (vs₁ ∪ vs₂)
 
 namespace Affine
 
-/-- How many times `x` occurs freely in `e`. -/
-def count (e : Affine vs) (x : String) : ℕ :=
+/-- The free variables in an affine term. -/
+abbrev free (_ : Affine vs) : Finset ℕ := vs
+
+/-- All variables in `e`. -/
+abbrev vars (e : Affine vs) : Finset ℕ :=
+  match e with
+  | .var x => {x}
+  | .abs x e => e.vars ∪ {x}
+  | .app e₁ e₂ _ => e₁.vars ∪ e₂.vars
+
+/-- Number of times `x` occurs freely in `e`. -/
+def count (e : Affine vs) (x : ℕ) : ℕ :=
   match e with
   | .var x' => if x = x' then 1 else 0
   | .abs x' e => if x = x' then 0 else count e x
   | .app e₁ e₂ _ => count e₁ x + count e₂ x
 
-/-- Affinity: Whether all variables occur at most once. -/
+/-- Whether all variables occur at most once. -/
 def is_affine (e : Affine vs) : Prop :=
   match e with
-  | .var x => True
+  | .var _ => True
   | .abs x e => is_affine e ∧ e.count x ≤ 1
   | .app e₁ e₂ _ => is_affine e₁ ∧ is_affine e₂ ∧ ∀ x, e₁.count x + e₂.count x ≤ 1
 
