Affine/Lambda.lean
@@ -1,0 +1,123 @@
+import Mathlib.Data.Nat.Basic
+import «Affine».Lemmas
+import «Affine».Misc
+
+inductive Lambda : Type
+| var (x : ℕ) : Lambda
+| abs (x : ℕ) (e : Lambda) : Lambda
+| app (e₁ : Lambda) (e₂ : Lambda) : Lambda
+
+namespace Lambda
+
+/-- Number of times `x` occurs freely in `e`. -/
+def count (e : Lambda) (x : ℕ) : ℕ :=
+  match e with
+  | .var x' => if x = x' then 1 else 0
+  | .abs x' e => if x = x' then 0 else count e x
+  | .app e₁ e₂ => count e₁ x + count e₂ x
+
+/-- Whether all variables occur at most once. -/
+def is_affine (e : Lambda) : Prop :=
+  match e with
+  | .var _ => True
+  | .abs x e => is_affine e ∧ e.count x ≤ 1
+  | .app e₁ e₂ => is_affine e₁ ∧ is_affine e₂ ∧ ∀ x, e₁.count x + e₂.count x ≤ 1
+
+def to_string (e : Lambda) : String :=
+  match e with
+  | .var x => s!"{x}"
+  | .abs x e => s!"(λ {x}. {e.to_string})"
+  | .app e₁ e₂ => s!"{e₁.to_string} {e₂.to_string}"
+
+end Lambda
+
+namespace Affine
+
+def to_lambda (e : Affine vs) : Lambda :=
+  match e with
+  | .var x => .var x
+  | .abs x e => .abs x e.to_lambda
+  | .app e₁ e₂ _ => .app e₁.to_lambda e₂.to_lambda
+
+theorem to_lambda_is_affine (e : Affine vs) : e.to_lambda.is_affine := by sorry
+
+theorem count_eq_to_lambda_count (e : Affine vs) : ∀ x, e.to_lambda.count x = e.count x := by
+  match e with
+  | .var x => simp only [Lambda.count, count, forall_const]
+  | .abs x e => simp_rw [Lambda.count, count, count_eq_to_lambda_count e, forall_const]
+  | .app e₁ e₂ h => simp_rw [Lambda.count, count, count_eq_to_lambda_count e₁,
+    count_eq_to_lambda_count e₂, forall_const]
+
+/--
+  `Affine` from `Lambda`.
+
+  We provide 3-tuple of the finset of free variables and a proof of equality `Affine.to_lambda`
+  as it's needed during induction for the `.app` case to produce the null_intersection argument
+  of `Affine.app`.
+-/
+def of_lambda_impl (e : Lambda) (he : e.is_affine) :
+    (vs : Finset ℕ) × (e' : Affine vs) ×' (e = e'.to_lambda) :=
+  match e with
+  | .var x => ⟨_, .var x, by simp only [to_lambda]⟩
+
+  | .abs x e =>
+    let ⟨e_free, e, he⟩ := of_lambda_impl e he.left
+    ⟨e_free \ {x}, .abs x e, by simp only [he, to_lambda]⟩
+
+  | .app e₁ e₂ =>
+    have ⟨h₁, h₂, h⟩ := he
+    let ⟨⟨e₁_free, e₁', he₁⟩, ⟨e₂_free, e₂', he₂⟩⟩ :=
+      (of_lambda_impl e₁ h₁, of_lambda_impl e₂ h₂)
+    have h_inter : e₁_free ∩ e₂_free = ∅ := by
+      simp_rw [he₁, he₂, count_eq_to_lambda_count] at h
+
+      by_contra h_inter
+      have ⟨v, hv⟩ := Finset.nonempty_of_ne_empty h_inter
+      have ⟨hv₁, hv₂⟩ := Finset.mem_inter.mp hv
+      have hv₁ := (count_ne_zero_iff e₁' v).mpr hv₁
+      have hv₂ := (count_ne_zero_iff e₂' v).mpr hv₂
+      exact Or.elim (Nat.add_le_one (h v)) hv₁ hv₂
+
+    have h_eq : Lambda.app e₁ e₂ = (Affine.app e₁' e₂' h_inter).to_lambda := by
+      simp only [he₁, he₂, to_lambda]
+
+    ⟨e₁_free ∪ e₂_free, .app e₁' e₂' h_inter, h_eq⟩
+
+def of_lambda (e : Lambda) (he : e.is_affine) : Affine (of_lambda_impl e he).1 :=
+  (Affine.of_lambda_impl e he).2.1
+
+theorem of_lambda_to_lambda (e : Lambda) (he : e.is_affine) :
+    e = (Affine.of_lambda e he).to_lambda := (of_lambda_impl e he).2.2
+
+theorem to_lambda_of_lambda_free (e : Affine vs) :
+  vs = (Affine.of_lambda e.to_lambda e.to_lambda_is_affine).free := by sorry
+
+-- theorem to_lambda_of_lambda (e : Affine vs) :
+--     e = to_lambda_of_lambda_free e ▸ (Affine.of_lambda e.to_lambda _) := by
+--   match e with
+--   | .var x => rfl
+--   | .abs x e =>
+--     have he := to_lambda_of_lambda e
+--     rw [of_lambda] at he
+--     simp_rw [to_lambda, of_lambda, of_lambda_impl, he]
+
+
+--   | .app e₁ e₂ h => sorry
+
+end Affine
+
+instance : ToString (Affine vs) := ⟨fun e => e.to_lambda.to_string⟩
+
+instance : ToString (Finset ℕ) := ⟨
+  let trans : IsTrans String (· < ·) := sorry
+  let trans : IsAntisymm String (· < ·) := sorry
+  let trans : IsTotal String (· < ·) := sorry
+  fun f => s!"\{{", ".intercalate (f.val.map ToString.toString |>.sort (· < ·))}}"
+⟩
+
+#eval (Affine.abs 1 (.app (.var 1) (.var 2) (by simp))) -- (λ 1. 1 2)
+
+#eval (Affine.abs 1 (.app (.var 1) (.var 2) (by simp))).vars -- {1, 2}
+
+-- next line will error since `1` occurs twice.
+-- #eval (Affine.abs 1 (.app (.var 1) (.var 1) (by simp)))
