Affine/Misc.lean
@@ -1,0 +1,3 @@
+import Mathlib.Data.Nat.Basic
+
+theorem Nat.add_le_one {a b : ℕ} : a + b ≤ 1 → a = 0 ∨ b = 0 := by sorry
